theories/L6_PCPS/Heap/space_sem.v
@@ -6,7 +6,7 @@ From Coq Require Import NArith.BinNat Relations.Relations MSets.MSets
          MSets.MSetRBT Lists.List omega.Omega Sets.Ensembles Relations.Relations
          Classes.Morphisms.
 From ExtLib Require Import Structures.Monad Data.Monads.OptionMonad Core.Type.
-From L6 Require Import cps cps_util eval List_util Ensembles_util functions
+From L6 Require Import cps ctx cps_util eval List_util Ensembles_util functions
         identifiers Heap.heap Heap.heap_defs Heap.heap_equiv tactics.
 Require Import compcert.lib.Coqlib.
 
@@ -20,229 +20,56 @@ Module SpaceSem (H : Heap).
 
   Import H Equiv.Defs Equiv.Defs.HL Equiv.
 
-  (* The cost of evaluating the head constructor before CC *)
-  Definition cost (e : exp) : nat :=
-    match e with
-      | Econstr x t ys e => 1 + length ys
-      | Ecase y cl => 1 
-      | Eproj x t n y e => 1
-      | Efun B e => fundefs_num_fv B + 1
-      | Eapp f t ys => 1 + length ys
-      | Eprim x p ys e => 1 + length ys
-      | Ehalt x => 1
+  Fixpoint def_funs (B B0 : fundefs) rho :=
+    match B with
+      | Fcons f _ _ _ B =>
+        M.set f (FunPtr B0 f) (def_funs B B0 rho)
+      | Fnil => rho
     end.
 
-  (* The cost of evaluating the head constructor after CC *)
-  Definition costCC (e : exp) : nat :=
+  (* The cost of evaluating the head constructor before CC *)
+  Definition cost (H : heap block) (rho : env) (e : exp) : nat :=
     match e with
       | Econstr x t ys e => 1 + length ys
       | Ecase y cl => 1 
       | Eproj x t n y e => 1
       | Efun B e => 1
       | Eapp f t ys => 1 + length ys
+        (* match M.get f rho with *)
+        (*   | Some (Loc l1) => *)
+        (*     match get l1 H with *)
+        (*       | Some (Clos (FunPtr B g) (Loc env_loc)) => *)
+        (*         match get env_loc H, find_def g B, getlist ys rho with *)
+        (*           | Some (Env rho_clo), Some (t, xs, e), Some vs => *)
+        (*             let '(H', rho_clo1) := def_closures B B rho_clo H env_loc in  *)
+        (*             match setlist xs vs rho_clo1 with *)
+        (*               | Some rho_clo2 =>  *)
+        (*                 1 + length ys + size_reachable (env_locs rho_clo2 (occurs_free e)) H *)
+        (*               | _ => 0 *)
+        (*             end *)
+        (*           | _,_ , _  => 0 *)
+        (*         end *)
+        (*       | _ => 0 *)
+        (*     end *)
+        (*   | Some (FunPtr B g) => *)
+        (*     match find_def g B,  getlist ys rho with *)
+        (*       | Some (ct, xs, e), Some vs => *)
+        (*         match setlist xs vs (def_funs B B (M.empty _)) with *)
+        (*           | Some rho_clo =>  *)
+        (*             1 + length ys + size_reachable (env_locs rho_clo (occurs_free e)) H *)
+        (*           | None => 0 *)
+        (*         end *)
+        (*       | _, _ => 0 *)
+        (*     end *)
+        (*   | None => 0 *)
+        (* end *)
       | Eprim x p ys e => 1 + length ys
       | Ehalt x => 1
     end.
   
-  
-  (** Non-deterministic semantics with garbage collection *)
-  Inductive big_step :
-    heap block -> (* The heap. Maps locations to values *)
-    env -> (* The environment. Maps variables to locations *)
-    exp -> (* The expression to be evaluated *)
-    ans -> (* The result of evaluation *)
-    nat -> (* Upper bound for the number of the evaluation steps *)
-    nat -> (* Maximum space required for the evaluation *)
-    Type := (* XXX This will bite us. Change it. *)
-  | Eval_oot : (* Out of time *)
-      forall (H : heap block) (rho : env) (e : exp) (c m : nat)
-        (Hsize : size_heap H = m)
-        (Hcost : c < cost e),
-        big_step H rho e OOT 0 m
-  | Eval_constr :
-      forall (H H' : heap block) (rho : env) (x : var) (t : cTag) (ys : list var)
-        (e : exp) (vs : list value) (l : loc) (r : ans) (c : nat) (m : nat)
-        (Hcost : c >= cost (Econstr x t ys e)) 
-        (Hget : getlist ys rho = Some vs)
-        (Halloc : alloc (Constr t vs) H = (l, H'))
-        (Hbs : big_step H' (M.set x (Loc l) rho) e r (c - cost (Econstr x t ys e)) m),
-        big_step H rho (Econstr x t ys e) r c m
-  | Eval_proj :
-      forall (H : heap block) (rho : env) (x : var) (t : cTag) (n : N) (y : var)
-        (e : exp) (l : loc) (v : value) (vs : list value) (r : ans) (c m : nat)
-        (Hcost : c >= cost (Eproj x t n y e))
-        (Hgety : M.get y rho = Some (Loc l))
-        (Hgetl : get l H = Some (Constr t vs)) 
-        (Hargs : nthN vs n = Some v)
-        (Hbs : big_step H (M.set x v rho) e r (c - cost (Eproj x t n y e)) m),
-        big_step H rho (Eproj x t n y e) r c m
-  | Eval_case :
-      forall (H : heap block) (rho : env) (y : var) (cl : list (cTag * exp))
-        (l : loc) (t : cTag) (vs : list value) (e : exp) (r : ans) (c m : nat)
-        (Hcost : c >= cost (Ecase y cl))
-        (Hgety : M.get y rho = Some (Loc l))
-        (Hgetl : get l H = Some (Constr t vs))
-        (Hfind : findtag cl t = Some e)
-        (Hbs : big_step H rho e r (c - cost (Ecase y cl)) m),
-        big_step H rho (Ecase y cl) r c m
-  | Eval_fun :
-      forall (H H' H'': heap block) (rho rho_clo rho' : env) (B : fundefs)
-        (env_loc : loc) (e : exp) (r : ans) (c : nat) (m : nat)
-        (Hcost : c >= cost (Efun B e))
-        (* find the closure environment *)
-        (Hres : Restrict_env (occurs_free_fundefs B) rho rho_clo)
-        (* allocate the closure environment *)
-        (Halloc : alloc (Env rho_clo) H = (env_loc, H'))
-        (* allocate the closures *)
-        (Hfuns : def_closures B B rho H' env_loc = (H'', rho'))
-        (Hbs : big_step H'' rho' e r (c - cost (Efun B e)) m),
-        big_step H rho (Efun B e) r c m
-  | Eval_app :
-      forall (H H' : heap block) (rho rho_clo rho_clo1 rho_clo2 : env) (B : fundefs)
-        (f f' : var) (t : cTag) (xs : list var) (e : exp) (l env_loc: loc)
-        (vs : list value) (ys : list var) (r : ans) (c : nat) (m : nat)
-        (Hcost : c >= cost (Eapp f t ys))
-        (Hgetf : M.get f rho = Some (Loc l))
-        (* Look up the closure *)
-        (Hgetl : get l H = Some (Clos (FunPtr B f') (Loc env_loc)))
-        (* Look up the closure environment *)
-        (Hget_env : get env_loc H = Some (Env rho_clo))
-        (* Find the code *)
-        (Hfind : find_def f' B = Some (t, xs, e))
-        (* Look up the actual parameters *)
-        (Hargs : getlist ys rho = Some vs)
-        (* Allocate mutually defined closures *)
-        (Hredef : def_closures B B rho_clo H env_loc = (H', rho_clo1))
-        (Hset : setlist xs vs rho_clo1 = Some rho_clo2)
-        (Hbs : big_step H' rho_clo2 e r (c - cost (Eapp f t ys)) m),
-        big_step H rho (Eapp f t ys) r c m
-  | Eval_halt :
-      forall (H : heap block) (rho : env) (x : var) (v : value) (c m : nat)
-        (Hcost : c >= cost (Ehalt x))
-        (Hget : M.get x rho = Some v)
-        (Heq : size_heap H = m),
-        big_step H rho (Ehalt x) (Res (v, H)) c m
-  | Eval_GC :
-      forall (H H' : heap block) (rho : env) (e : exp) (r : ans) (c : nat) (m m' : nat)
-        (* Garbage collect H *)
-        (Hgc : collect (env_locs rho (occurs_free e)) H H')
-        (* XXX cost model? *)
-        (Hsize : H.size H' = m' -> c >= m')
-        (Hbs : big_step H' rho e r (c - m') m),
-        big_step H rho e r c (max m m').
-  
-  (** Deterministic semantics with perfect garbage collection
-   * The execution time cost model does not account for the cost of GC  *)
-  Inductive big_step_perfect_GC :
-    heap block -> (* The heap. Maps locations to values *)
-    env -> (* The environment. Maps variables to locations *)
-    exp -> (* The expression to be evaluated *)
-    ans -> (* The final result, which is a pair of a location an a heap *)
-    nat -> (* Upper bound for the number of the evaluation steps  *)
-    nat -> (* The maximum space required for the evaluation *)
-    Prop :=
-  | Eval_oot_per :
-      forall (H : heap block) (rho : env) (e : exp) (c m : nat)
-        (Hcost : c < cost e) 
-        (Hsize : size_heap H = m),
-        (big_step_perfect_GC H rho e OOT c m)
-  | Eval_constr_per :
-      forall (H H' H'' : heap block) (rho rho' : env) (x : var) (t : cTag)
-        (ys :list var) (e : exp) (vs : list value) (l : loc) (r : ans)
-        (c m m' : nat)
-        (Hcost :  c >= cost (Econstr x t ys e))
-        (Hget : getlist ys rho = Some vs)
-        (Halloc : alloc (Constr t vs) H = (l, H'))
-        
-        (* collect H' *)
-        (Hgc : live (env_locs (M.set x (Loc l) rho) (occurs_free e)) H' H'')
-        (Hsize : size_heap H' = m')
-        
-        (Hbs : big_step_perfect_GC H'' (M.set x (Loc l) rho) e r (c - cost (Econstr x t ys e)) m),
-
-        big_step_perfect_GC H rho (Econstr x t ys e) r c (max m m')
-  | Eval_proj_per :
-      forall (H H' : heap block) (rho : env) (x : var) (t : cTag) (n : N)
-        (y : var) (e : exp) (l : loc) (v : value) (vs : list value)
-        (r : ans) (c m m' : nat)
-        (Hcost : c >= cost (Eproj x t n y e))
-        (Hgety : M.get y rho = Some (Loc l))
-        (Hgetl : get l H = Some (Constr t vs))
-        (Hnth : nthN vs n = Some v)
-
-        (* collect H *)
-        (Hgc : live (env_locs (M.set x v rho) (occurs_free e)) H H')
-        (Hsize : size_heap H = m')
-
-        (Hbs : big_step_perfect_GC H' (M.set x v rho) e r (c - 1) m),
-        
-        big_step_perfect_GC H rho (Eproj x t n y e) r c (max m m')
-  | Eval_case_per :
-      forall (H H' : heap block) (rho : env) (y : var) (cl : list (cTag * exp))
-        (l : loc) (t : cTag) (vs : list value) (e : exp) (r : ans) (c m m' : nat)
-        (Hcost : c >= cost (Ecase y cl))
-        (Hgety : M.get y rho = Some (Loc l))
-        (Hgetl : get l H = Some (Constr t vs))
-        (Htag : findtag cl t = Some e)
-
-        (* collect H *)
-        (Hgc : live ((env_locs rho) (occurs_free e)) H H')
-        (Hsize : size_heap H = m')
-
-        (Hbs : big_step_perfect_GC H' rho e r (c - cost (Ecase y cl)) m),
-        
-        big_step_perfect_GC H rho (Ecase y cl) r c (max m m')
-  | Eval_fun_per :
-      forall (H H' H'' H''': heap block) (rho rho_clo rho' : env) (B : fundefs)
-        (env_loc : loc) (e : exp) (r : ans) (c : nat) (m m' : nat)
-        (Hcost : c >= cost (Efun B e))
-        (* find the closure environment *)
-        (Hres : restrict_env (fundefs_fv B) rho = rho_clo)
-        (* allocate the closure environment *)
-        (Halloc : alloc (Env rho_clo) H = (env_loc, H'))
-        (* allocate the closures *)
-        (Hfuns : def_closures B B rho H' env_loc = (H'', rho'))
-
-        (* collect H'' *)
-        (Hgc : live (env_locs rho' (occurs_free e)) H'' H''')
-        (Hsize : size_heap H'' = m')
-
-        (Hbs : big_step_perfect_GC H''' rho' e r (c - cost (Efun B e)) m),
-        big_step_perfect_GC H rho (Efun B e) r c (max m m')
-    
-  | Eval_app_per :
-      forall (H H' H'' : heap block) (rho rho_clo rho_clo1 rho_clo2 : env) (B : fundefs)
-        (f f' : var) (t : cTag) (xs : list var) (e : exp) (l env_loc: loc)
-        (vs : list value) (ys : list var) (r : ans) (c : nat) (m m' : nat)
-        (Hcost : c >= cost (Eapp f t ys))
-        (Hgetf : M.get f rho = Some (Loc l))
-        (* Look up the closure *)
-        (Hgetl : get l H = Some (Clos (FunPtr B f') (Loc env_loc)))
-        (* Look up the closure environment *)
-        (Hget_env : get env_loc H = Some (Env rho_clo))
-        (* Find the code *)
-        (Hfind : find_def f' B = Some (t, xs, e))
-        (* Look up the actual parameters *)
-        (Hargs : getlist ys rho = Some vs)
-        (* Allocate mutually defined closures *)
-        (Hredef : def_closures B B rho_clo H env_loc = (H', rho_clo1))
-        (Hset : setlist xs vs rho_clo1 = Some rho_clo2)
-        
-        (* collect H' *)
-        (Hgc : live ((env_locs rho_clo2) (occurs_free e)) H' H'')
-        (Hsize : size_heap H' = m')
-        
-        (Hbs : big_step_perfect_GC H'' rho_clo2 e r (c - cost (Eapp f t ys)) m),
-        big_step_perfect_GC H rho (Eapp f t ys) r c (max m m')
-  | Eval_halt_per :
-      forall H rho x l c m
-        (Hcost : c >= cost (Ehalt x))
-        (Hget : M.get x rho = Some l)
-        (Hsize : size_heap H = m),
-        big_step_perfect_GC H rho (Ehalt x) (Res (l, H)) c m.
-
   (** Deterministic semantics with garbage collection upon function entry.
-    * We will show that it takes asymptotically the same amount of space as perfect garbage collection *)
+    * We will show that it takes asymptotically the same amount of space as perfect
+    * garbage collection. *)
   Inductive big_step_GC :
     heap block -> (* The heap. Maps locations to values *)
     env -> (* The environment. Maps variables to locations *)
@@ -253,47 +80,47 @@ Module SpaceSem (H : Heap).
     Prop :=
   | Eval_oot_gc :
       forall (H : heap block) (rho : env) (e : exp) (c m : nat)
-        (Hcost : c < cost e) 
+        (Hcost : c < cost H rho e) 
         (Hsize : size_heap H = m),
         (big_step_GC H rho e OOT c m)
   | Eval_constr_gc :
       forall (H H' : heap block) (rho rho' : env) (x : var) (t : cTag)
         (ys : list var) (e : exp) (vs : list value) (l : loc) (r : ans)
         (c m : nat)
-        (Hcost :  c >= cost (Econstr x t ys e))
+        (Hcost :  c >= cost H rho (Econstr x t ys e))
         (Hget : getlist ys rho = Some vs)
         (Halloc : alloc (Constr t vs) H = (l, H'))
                 
-        (Hbs : big_step_GC H' (M.set x (Loc l) rho) e r (c - cost (Econstr x t ys e)) m),
+        (Hbs : big_step_GC H' (M.set x (Loc l) rho) e r (c - cost H rho (Econstr x t ys e)) m),
 
         big_step_GC H rho (Econstr x t ys e) r c m
   | Eval_proj_gc : (* XXX Tag annotation in projections is redundant in this semantics *)
       forall (H : heap block) (rho : env) (x : var) (t t' : cTag) (n : N)
         (y : var) (e : exp) (l : loc) (v : value) (vs : list value)
         (r : ans) (c m : nat)
-        (Hcost : c >= cost (Eproj x t n y e))
+        (Hcost : c >= cost H rho (Eproj x t n y e))
         (Hgety : M.get y rho = Some (Loc l))
         (Hgetl : get l H = Some (Constr t' vs))
         (Hnth : nthN vs n = Some v)
         
-        (Hbs : big_step_GC H (M.set x v rho) e r (c - 1) m),
+        (Hbs : big_step_GC H (M.set x v rho) e r (c - cost H rho (Eproj x t n y e)) m),
         
         big_step_GC H rho (Eproj x t n y e) r c m
   | Eval_case_gc :
       forall (H : heap block) (rho : env) (y : var) (cl : list (cTag * exp))
         (l : loc) (t : cTag) (vs : list value) (e : exp) (r : ans) (c m : nat)
-        (Hcost : c >= cost (Ecase y cl))
+        (Hcost : c >= cost H rho (Ecase y cl))
         (Hgety : M.get y rho = Some (Loc l))
         (Hgetl : get l H = Some (Constr t vs))
         (Htag : findtag cl t = Some e)
         
-        (Hbs : big_step_GC H rho e r (c - cost (Ecase y cl)) m),
+        (Hbs : big_step_GC H rho e r (c - cost H rho (Ecase y cl)) m),
         
         big_step_GC H rho (Ecase y cl) r c m
   | Eval_fun_gc :
       forall (H H' H'' : heap block) (rho rho_clo rho' : env) (B : fundefs)
         (env_loc : loc) (e : exp) (r : ans) (c : nat) (m : nat)
-        (Hcost : c >= cost (Efun B e))
+        (Hcost : c >= cost H rho (Efun B e))
         (* find the closure environment *)
         (Hres : restrict_env (fundefs_fv B) rho = rho_clo)
         (* allocate the closure environment *)
@@ -301,7 +128,7 @@ Module SpaceSem (H : Heap).
         (* allocate the closures *)
         (Hfuns : def_closures B B rho H' env_loc = (H'', rho'))
         
-        (Hbs : big_step_GC H'' rho' e r (c - cost (Efun B e)) m),
+        (Hbs : big_step_GC H'' rho' e r (c - cost H rho (Efun B e)) m),
 
         big_step_GC H rho (Efun B e) r c m
     
@@ -309,7 +136,7 @@ Module SpaceSem (H : Heap).
       forall (H H' H'' : heap block) (rho rho_clo rho_clo1 rho_clo2 : env) (B : fundefs)
         (f f' : var) (t : cTag) (xs : list var) (e : exp) (l env_loc: loc)
         (vs : list value) (ys : list var) (r : ans) (c : nat) (m m' : nat)
-        (Hcost : c >= cost (Eapp f t ys))
+        (Hcost : c >= cost H rho (Eapp f t ys))
         (Hgetf : M.get f rho = Some (Loc l))
         (* Look up the closure *)
         (Hgetl : get l H = Some (Clos (FunPtr B f') (Loc env_loc)))
@@ -327,22 +154,15 @@ Module SpaceSem (H : Heap).
         (Hgc : live ((env_locs rho_clo2) (occurs_free e)) H' H'')
         (Hsize : size_heap H' = m')
         
-        (Hbs : big_step_GC H'' rho_clo2 e r (c - cost (Eapp f t ys)) m),
+        (Hbs : big_step_GC H'' rho_clo2 e r (c - cost H rho (Eapp f t ys)) m),
         big_step_GC H rho (Eapp f t ys) r c (max m m')
   | Eval_halt_gc :
       forall H rho x l c m
-        (Hcost : c >= cost (Ehalt x))
+        (Hcost : c >= cost H rho (Ehalt x))
         (Hget : M.get x rho = Some l)
         (Hsize : size_heap H = m),
         big_step_GC H rho (Ehalt x) (Res (l, H)) c m.
 
-
-  Fixpoint def_funs (B B0 : fundefs) rho :=
-    match B with
-      | Fcons f _ _ _ B =>
-        M.set f (FunPtr B0 f) (def_funs B B0 rho)
-      | Fnil => rho
-    end.
 
   (** Deterministic semantics with perfect garbage collection, for closure converted code
    * The execution time cost model does not account for the cost of GC  *)
@@ -356,59 +176,59 @@ Module SpaceSem (H : Heap).
     Prop :=
   | Eval_oot_per_cc :
       forall (H : heap block) (rho : env) (e : exp) (c m : nat)
-        (Hcost : c < costCC e) 
+        (Hcost : c < cost H rho e) 
         (Hsize : size_heap H = m),
         (big_step_GC_cc H rho e OOT c m)
   | Eval_constr_per_cc :
       forall (H H' : heap block) (rho : env) (x : var) (t : cTag)
         (ys :list var) (e : exp) (vs : list value) (l : loc) (r : ans)
         (c m : nat)
-        (Hcost :  c >= costCC (Econstr x t ys e))
+        (Hcost :  c >= cost H rho (Econstr x t ys e))
         (Hget : getlist ys rho = Some vs)
         (Halloc : alloc (Constr t vs) H = (l, H'))
               
-        (Hbs : big_step_GC_cc H' (M.set x (Loc l) rho) e r (c - costCC (Econstr x t ys e)) m),
+        (Hbs : big_step_GC_cc H' (M.set x (Loc l) rho) e r (c - cost H rho (Econstr x t ys e)) m),
 
         big_step_GC_cc H rho (Econstr x t ys e) r c m
   | Eval_proj_per_cc : (* XXX Tag annotation in projections is redundant in this semantics *)
       forall (H : heap block) (rho : env) (x : var) (t t' : cTag) (n : N)
         (y : var) (e : exp) (l : loc) (v : value) (vs : list value)
         (r : ans) (c m : nat)
-        (Hcost : c >= costCC (Eproj x t n y e))
+        (Hcost : c >= cost H rho (Eproj x t n y e))
         (Hgety : M.get y rho = Some (Loc l))
         (Hgetl : get l H = Some (Constr t' vs))
         (Hnth : nthN vs n = Some v)
 
-        (Hbs : big_step_GC_cc H (M.set x v rho) e r (c - 1) m),
+        (Hbs : big_step_GC_cc H (M.set x v rho) e r (c - cost H rho (Eproj x t n y e)) m),
         
         big_step_GC_cc H rho (Eproj x t n y e) r c m
   | Eval_case_per_cc :
       forall (H H' : heap block) (rho : env) (y : var) (cl : list (cTag * exp))
         (l : loc) (t : cTag) (vs : list value) (e : exp) (r : ans) (c m : nat)
-        (Hcost : c >= costCC (Ecase y cl))
+        (Hcost : c >= cost H rho (Ecase y cl))
         (Hgety : M.get y rho = Some (Loc l))
         (Hgetl : get l H = Some (Constr t vs))
         (Htag : findtag cl t = Some e)
 
 
-        (Hbs : big_step_GC_cc H' rho e r (c - costCC (Ecase y cl)) m),
+        (Hbs : big_step_GC_cc H' rho e r (c - cost H rho (Ecase y cl)) m),
         
         big_step_GC_cc H rho (Ecase y cl) r c m
   | Eval_fun_per_cc :
       forall (H : heap block) (rho rho' : env) (B : fundefs)
         (e : exp) (r : ans) (c : nat) (m : nat)
-        (Hcost : c >= costCC (Efun B e))
+        (Hcost : c >= cost H rho (Efun B e))
         (* add the functions in the environment *)
         (Hfuns : def_funs B B rho = rho')
         
-        (Hbs : big_step_GC_cc H rho' e r (c - costCC (Efun B e)) m),
+        (Hbs : big_step_GC_cc H rho' e r (c - cost H rho (Efun B e)) m),
         
         big_step_GC_cc H rho (Efun B e) r c m
   | Eval_app_per_cc :
       forall (H H' : heap block) (rho rho_clo : env) (B : fundefs)
         (f f' : var) (ct : cTag) (xs : list var) (e : exp)
         (vs : list value) (ys : list var) (r : ans) (c : nat) (m m' : nat)
-        (Hcost : c >= costCC (Eapp f ct ys))
+        (Hcost : c >= cost H rho (Eapp f ct ys))
         (Hgetf : M.get f rho = Some (FunPtr B f'))
         (* Find the code *)
         (Hfind : find_def f' B = Some (ct, xs, e))
@@ -420,151 +240,23 @@ Module SpaceSem (H : Heap).
         (Hgc : live' ((env_locs rho_clo) (occurs_free e)) H H')
         (Hsize : size_heap H = m')
         
-        (Hbs : big_step_GC_cc H' rho_clo e r (c - costCC (Eapp f ct ys)) m),
+        (Hbs : big_step_GC_cc H' rho_clo e r (c - cost H rho (Eapp f ct ys)) m),
         big_step_GC_cc H rho (Eapp f ct ys) r c (max m m')
   | Eval_halt_per_cc :
       forall H rho x l c m
-        (Hcost : c >= costCC (Ehalt x))
+        (Hcost : c >= cost H rho (Ehalt x))
         (Hget : M.get x rho = Some l)
         (Hsize : size_heap H = m),
         big_step_GC_cc H rho (Ehalt x) (Res (l, H)) c m.
   
-  (** Deterministic semantics with garbage collection when needed.
-   * The execution time cost model accounts for the cost of GC  *)
-  Context (Hmax : nat).
-  
-  Inductive big_step_GC_when_needed :
-    heap block -> (* The heap. Maps locations to values *)
-    env -> (* The environment. Maps variables to locations *)
-    exp -> (* The expression to be evaluated *)
-    ans -> (* The final result, which is a pair of a location an a heap *)
-    nat -> (* Upper bound for the number of the evaluation steps  *)
-    nat -> (* The maximum space required for the evaluation *)
-    Prop :=
-  | Eval_constr_need :
-      forall (H H' : heap block) (rho rho' : env) (x : var) (t : cTag) (ys :list var)
-        (e : exp) (vs : list value) (l : loc) (r : ans) (c m : nat),
-        c >= cost (Econstr x t ys e) ->
-        (* No GC is needed *)
-        size_heap H < Hmax ->
-        
-        getlist ys rho = Some vs ->
-        alloc (Constr t vs) H = (l, H') ->
-        big_step_GC_when_needed H' (M.set x (Loc l) rho) e r (c - cost (Econstr x t ys e)) m ->
-        big_step_GC_when_needed H rho (Econstr x t ys e) r c m
-  | Eval_proj_need :
-      forall (H : heap block) (rho : env) (x : var) (t : cTag) (n : N)
-        (y : var) (e : exp) (l : loc) (v : value) (vs : list value)
-        (r : ans) (c m : nat),
-        c >= cost (Eproj x t n y e) ->
-        (* No GC is needed *)
-        size_heap H < Hmax ->
-        
-        M.get y rho = Some (Loc l) ->
-        get l H = Some (Constr t vs) -> 
-        nthN vs n = Some v ->
-        big_step_GC_when_needed H (M.set x v rho) e r (c - cost (Eproj x t n y e)) m ->
-        big_step_GC_when_needed H rho (Eproj x t n y e) r c m
-  | Eval_case_need :
-      forall (H : heap block) (rho : env) (y : var) (cl : list (cTag * exp))
-        (l : loc) (t : cTag) (vs : list value)
-        (e : exp) (r : ans) (size c m : nat),
-        c >= cost (Ecase y cl) ->
-        (* No GC is needed *)
-        size_heap H < Hmax ->
-
-        M.get y rho = Some (Loc l) ->
-        get l H = Some (Constr t vs) ->
-        findtag cl t = Some e ->
-        big_step_GC_when_needed H rho e r (c - cost (Ecase y cl)) m ->
-        big_step_GC_when_needed H rho (Ecase y cl) r c m
-  | Eval_fun_need :
-      forall (H H' H'' : heap block) (rho rho_clo rho' : env) (B : fundefs)
-        (env_loc : loc) (e : exp) (r : ans) (size c m : nat)
-        (Hcost: c >= cost (Efun B e))
-        (* No GC is needed *)
-        (Hheap : size_heap H < Hmax)
-        (* find the closure environment *)
-        (Hres : restrict_env (fundefs_fv B) rho = rho_clo)
-        (* allocate the closure environment *)
-        (Halloc : alloc (Env rho_clo) H = (env_loc, H'))
-        (* allocate the closures *)
-        (Hfuns : def_closures B B rho H' env_loc = (H'', rho'))
-        (Hbs : big_step_GC_when_needed H'' rho' e r (c - cost (Efun B e)) m),
-        big_step_GC_when_needed H rho (Efun B e) r c m
-  | Eval_app_need :
-      forall (H H' : heap block) (rho rho_clo rho_clo1 rho_clo2 : env) (B : fundefs)
-        (f f' : var) (t : cTag) (xs : list var) (e : exp) (l env_loc: loc)
-        (vs : list value) (ys : list var) (r : ans) (c : nat) (m : nat)
-        (Hcost : c >= cost (Eapp f t ys))
-        (* No GC is needed *)
-        (Hheap : size_heap H < Hmax)
-        (Hgetf : M.get f rho = Some (Loc l))
-        (* Look up the closure *)
-        (Hgetl : get l H = Some (Clos (FunPtr B f') (Loc env_loc)))
-        (* Look up the closure environment *)
-        (Hget_env : get env_loc H = Some (Env rho_clo))
-        (* Find the code *)
-        (Hfind : find_def f' B = Some (t, xs, e))
-        (* Look up the actual parameters *)
-        (Hargs : getlist ys rho = Some vs)
-        (* Allocate mutually defined closures *)
-        (Hredef : def_closures B B rho_clo H env_loc = (H', rho_clo1))
-        (Hset : setlist xs vs rho_clo1 = Some rho_clo2)
-        (Hbs : big_step_GC_when_needed H' rho_clo2 e r (c - cost (Eapp f t ys)) m),
-        big_step_GC_when_needed H rho (Eapp f t ys) r c m
-  | Eval_halt_need :
-      forall (H : heap block) (rho : env) (x : var) (v : value) (c m : nat),
-        c >= cost (Ehalt x) ->
-        M.get x rho = Some v ->
-        size_heap H = m ->
-        big_step_GC_when_needed H rho (Ehalt x) (Res (v, H)) c m
-  | Eval_GC_need :
-      forall (H H' : heap block) (rho : env) (e : exp) (r : ans) (c : nat) (m m' : nat),
-        (* Garbage collect H *)
-        live (env_locs rho (occurs_free e)) H H' ->
-        size_heap H' = m' ->
-        (* Collect only if it's needed *)
-        Hmax <= m' ->
-        c >= m' ->
-        big_step_GC_when_needed H' rho e r (c - m') m ->
-        big_step_GC_when_needed H rho e r c (max m m').
-  
-  Fixpoint noGC {Heap rho e v c m} (H : big_step Heap rho e v c m) : Prop :=
-    match H with
-      | Eval_oot H rho e c m Hsize Hcost => True
-      | Eval_constr H H' rho x t ys e vs l r c m Hcost Hget Halloc Hbs => noGC Hbs
-      | Eval_proj H rho x t n y e l v vs r c m Hcost Hgety Hgetl Hargs Hbs => noGC Hbs
-      | Eval_case H rho y cl l t vs e r c m Hcost Hgety Hgetl Hfind Hbs => noGC Hbs
-      | Eval_fun H H' H'' rho rho_clo rho' B env_loc e r c m Hcost Hres Halloc
-                 Hfuns Hbs => noGC Hbs
-      | Eval_app H H' rho rho_clo rho_clo1 rho_clo2 B f f' t xs e l env_loc vs
-                 ys r c m Hcost Hgetf Hgetl Hget_env Hfind Hargs Hredef Hset Hbs => noGC Hbs
-      | Eval_halt H rho x v c m Hcost Hget Heq => True
-      | Eval_GC H H' rho e r c m m' Hgc Hsize Hbs => False
-    end.
-  
-  (** Size of the [big_step] derivation *)
-  Fixpoint size_big_step {Heap rho e v c m} (H : big_step Heap rho e v c m) : nat :=
-    match H with
-      | Eval_oot H rho e c m Hsize Hcost => 0
-      | Eval_constr H H' rho x t ys e vs l r c m Hcost Hget Halloc Hbs => 1 + size_big_step Hbs
-      | Eval_proj H rho x t n y e l v vs r c m Hcost Hgety Hgetl Hargs Hbs => 1 + size_big_step Hbs
-      | Eval_case H rho y cl l t vs e r c m Hcost Hgety Hgetl Hfind Hbs => 1 + size_big_step Hbs
-      | Eval_fun H H' H'' rho rho_clo rho' B env_loc e r c m Hcost Hres Halloc
-                 Hfuns Hbs => 1 + size_big_step Hbs
-      | Eval_app H H' rho rho_clo rho_clo1 rho_clo2 B f f' t xs e l env_loc vs
-                 ys r c m Hcost Hgetf Hgetl Hget_env Hfind Hargs Hredef Hset Hbs => 1 + size_big_step Hbs
-      | Eval_halt H rho x v c m Hcost Hget Heq => 0
-      | Eval_GC H H' rho e r c m m' Hgc Hsize Hbs => S (size_big_step Hbs)
-    end.
 
   Definition is_res (r : ans) : Prop :=
     match r with
       | Res _ =>  True
       | _ => False
     end.
-
+  
+  (* TODO move *)
   Definition reach_ans (a : ans) : Ensemble loc :=
     match a with
       | Res r => reach_res r
@@ -572,7 +264,7 @@ Module SpaceSem (H : Heap).
       | OOM => Empty_set _
     end.
   
-  Lemma big_step_gc_heap_env_equiv H1 H2 β rho1 rho2 e (r : ans) c m :
+  Lemma big_step_gc_heap_env_equiv_l H1 H2 β rho1 rho2 e (r : ans) c m :
     big_step_GC H1 rho1 e r c m ->
     (occurs_free e) |- (H1, rho1) ⩪_(β, id) (H2, rho2) ->
     injective_subdomain (reach' H1 (env_locs rho1 (occurs_free e))) β -> 
@@ -580,8 +272,8 @@ Module SpaceSem (H : Heap).
                  injective_subdomain (reach_ans r') β' /\
                  ans_equiv β' r id r').
   Admitted.
-
-  Lemma big_step_gc_heap_env_equiv2 H1 H2 β1 β2 rho1 rho2 e (r : ans) c m :
+  
+  Lemma big_step_gc_heap_env_equiv_r H1 H2 β1 β2 rho1 rho2 e (r : ans) c m :
     big_step_GC H1 rho1 e r c m ->
     (occurs_free e) |- (H1, rho1) ⩪_(β1, β2) (H2, rho2) ->
     injective_subdomain (reach' H1 (env_locs rho1 (occurs_free e))) β1 ->
@@ -592,563 +284,171 @@ Module SpaceSem (H : Heap).
                       ans_equiv β1' r β2' r').
   Admitted.
 
+
+  (** * Interpretation of a context as a heap and an environment *)
+
+  Fixpoint costCC_ctx_full (c : exp_ctx) : nat :=
+    match c with
+      | Econstr_c x t ys c => 1 + length ys + costCC_ctx_full c
+      | Eproj_c x t n y c => 1 + costCC_ctx_full c
+      | Efun1_c B c => 1 + costCC_ctx_full c
+      | Eprim_c x p ys c => 1 + length ys + costCC_ctx_full c
+      | Hole_c => 0
+      | Efun2_c _ _ => 0 (* maybe fix but not needed for now *)
+      | Ecase_c _ _ _ _ _ => 0
+    end.
   
-  (* 
-  Lemma big_step_deterministic  H1 H2 rho1 rho2 e r1 r1' c1 m1 r2 r2' c2 m2 :
-    well_formed (reach' H1 (env_locs rho1 (occurs_free e))) H1 ->
-    well_formed (reach' H2 (env_locs rho2 (occurs_free e))) H2 ->
-    env_locs rho1 (occurs_free e) \subset dom H1 ->
-    env_locs rho2 (occurs_free e) \subset dom H2 ->
-    big_step H1 rho1 e r1 c1 m1 -> (* D1 *)
-    big_step H2 rho2 e r2 c2 m2 -> (* D2 *)
-    r1 = Res r1' -> r2 = Res r2' ->
-    (occurs_free e) |- (H1, rho1) ⩪ (H2, rho2) ->
-     r1' ≈ r2'.
-  Proof with now eauto with Ensembles_DB.
-    (* Lexicographic induction on the size of the first derivation and the size of the second derivation *)
-    intros Hwf1 Hwf2 Hwfe1 Hwfe2 Hbs1 Hbs2. remember (size_big_step Hbs1) as n.
-    revert H1 H2 rho1 rho2 e r1 r1' c1 m1 r2 r2' c2 m2 Hwf1 Hwf2 Hwfe1 Hwfe2 Hbs1 Heqn Hbs2.
-    induction n as [n IH1] using lt_wf_rec1.
-    intros H1 H2 rho1 rho2 e r1 r1' c1 m1 r2 r2' c2 m2 Hwf1 Hwf2 Hwfe1 Hwfe2 Hbs1 Heqn Hbs2.
-    subst.
-    remember (size_big_step Hbs2) as m.
-    revert H1 H2 rho1 rho2 e r1 r1' c1 m1 r2 r2' c2 m2 Hwf1 Hwf2 Hwfe1 Hwfe2 Hbs1 Hbs2 Heqm IH1.
-    induction m as [m IH2] using lt_wf_rec1.  
-    intros H1 H2 rho1 rho2 e r1 r1' c1 m1 r2 r2' c2 m2 Hwf1 Hwf2 Hwfe1 Hwfe2 Hbs1 Hbs2
-           Heqm IH1 Heq1 Heq2 Heq.
-    
-    destruct Hbs1; simpl in *.
-    - (* D1 : OOT *) discriminate.
-    - (* D1 : Eval_constr *)
-      subst m. remember (Econstr x t ys e) as e'. destruct Hbs2; inv Heqe'; simpl in *.
-      + (* D2 : OOT *) discriminate.
-      + (* D2 : Eval_constr *)
-        subst.
-        eapply IH1 with (Hbs1 := Hbs1);
-          [ | | | | | reflexivity | | reflexivity | reflexivity |]. 
-        * omega.
-        * eapply well_formed_antimon. eapply reach'_set_monotonic.
-          eapply env_locs_monotonic. now apply occurs_free_Econstr_Included.
-          eapply well_formed_reach_alloc with (H := H); eauto.
-          eapply Included_trans; [| now apply reach'_extensive ].
-          simpl. eapply FromList_env_locs; eauto. normalize_occurs_free...
-        * eapply well_formed_antimon. eapply reach'_set_monotonic.
-          eapply env_locs_monotonic. now apply occurs_free_Econstr_Included.
-          eapply well_formed_reach_alloc with (H := H0) (l := l0); eauto.
-          eapply Included_trans; [| now apply reach'_extensive ].
-          simpl. eapply FromList_env_locs; eauto. normalize_occurs_free...
-        * eapply Included_trans.
-          eapply env_locs_monotonic. now apply occurs_free_Econstr_Included.
-          eapply Included_trans. eapply env_locs_set_Inlcuded.
-          eapply Union_Included. eapply Singleton_Included.
-          now eapply alloc_In_dom; eauto.
-          eapply Included_trans. eassumption.
-          eapply dom_subheap. now eapply alloc_subheap; eauto.
-        * eapply Included_trans.
-          eapply env_locs_monotonic. now apply occurs_free_Econstr_Included.
-          eapply Included_trans. eapply env_locs_set_Inlcuded.
-          eapply Union_Included. eapply Singleton_Included.
-          now eapply alloc_In_dom; eauto.
-          eapply Included_trans. eassumption.
-          eapply dom_subheap. now eapply alloc_subheap; eauto.
-        * eassumption.
-        * eapply (heap_env_equiv_alloc _ _ _ H H0); eauto. 
-          eapply reach'_closed. eassumption. eassumption.
-          eapply reach'_closed. eassumption. eassumption.
-          eapply Included_trans; [| now apply reach'_extensive ].
-          eapply env_locs_monotonic. normalize_occurs_free...
-          eapply Included_trans; [| now apply reach'_extensive ].
-          eapply env_locs_monotonic. normalize_occurs_free...
-          eapply Included_trans; [| now apply reach'_extensive ].
-          eapply FromList_env_locs; eauto. normalize_occurs_free...
-          eapply Included_trans; [| now apply reach'_extensive ].
-          eapply FromList_env_locs; eauto. normalize_occurs_free...
-          eapply heap_env_equiv_antimon. eassumption.
-          eapply Setminus_Included_Included_Union. now eapply occurs_free_Econstr_Included.
-          split. reflexivity.
-          eapply Forall2_symm_strong; [| eapply heap_env_equiv_getlist_Forall2 ].
-          intros. now symmetry. now split; eapply Heq.
-          rewrite occurs_free_Econstr... eassumption. eassumption.
-      + (* D2 : Eval_GC *)
-        assert (Hex : exists  (Hbs1' : big_step H rho (Econstr x t ys e) (Res r1') c m0),
-                        size_big_step Hbs1' = S (size_big_step Hbs1)).
-        { exists (Eval_constr H H' rho x t ys e vs l (Res r1') c m0 Hcost Hget Halloc Hbs1).
-          reflexivity. }
-        destruct Hex as [Hbs1' Hsize']. 
-        eapply IH2 with (Hbs2 := Hbs2) (Hbs1 := Hbs1');
-          [ | | | | | reflexivity | | reflexivity | reflexivity |]; try eassumption.
-        * omega. 
-        * eapply heap_equiv_respects_well_formed; [| eassumption ].
-          destruct Hgc as [_ Hequiv]. exact Hequiv.
-        * eapply heap_equiv_in_dom.
-          destruct Hgc as [_ Hequiv]. exact Hequiv.
-          reflexivity. eassumption.
-        * intros. subst. eapply IH1 with (Hbs1 := Hbs0);
-            [| | | | | reflexivity | | reflexivity | reflexivity | ]; try eassumption.
-          omega.
-        * edestruct Equivalence_heap_env_equiv. eapply Equivalence_Transitive; eauto.
-          eapply heap_env_equiv_heap_equiv.
-          eapply collect_heap_eq. eassumption.
-    - (* D1 : Eval_proj *)
-      subst m. remember (Eproj x t n y e) as e'. destruct Hbs2; inv Heqe'; simpl in *.
-      + (* D2 : OOT *) discriminate.
-      + (* D2 : Eval_proj *)
-        eapply IH1 with (Hbs1 := Hbs1); [ | | | | | reflexivity | | reflexivity | reflexivity |];
-        try eassumption.
-        * omega.
-        * eapply well_formed_antimon. eapply reach'_set_monotonic.
-          eapply Included_trans.
-          eapply env_locs_monotonic. now apply occurs_free_Eproj_Included.
-          eapply env_locs_set_Inlcuded.
-          rewrite <-reach_spec. eassumption. now eauto with Ensembles_DB.
-          eapply Union_Included.
-          intros l1 Hin. eexists 1.
-          split. now constructor. eexists l. eexists.
-          repeat split; eauto; simpl. eexists; split; eauto.
-          now rewrite Hgety. eapply In_Union_list; [| eassumption ].
-          eapply in_map. now eapply nthN_In; eauto.
-          now apply reach'_extensive.
-        * eapply well_formed_antimon. eapply reach'_set_monotonic.
-          eapply Included_trans.
-          eapply env_locs_monotonic. now apply occurs_free_Eproj_Included.
-          eapply env_locs_set_Inlcuded.
-          rewrite <-reach_spec. eassumption. now eauto with Ensembles_DB.
-          eapply Union_Included.
-          intros l1 Hin. eexists 1. split.
-          now constructor.
-          eexists l0. eexists. repeat split; eauto; simpl.
-          eexists; split; eauto.
-          now rewrite Hgety0. eapply In_Union_list; [| eassumption ].
-          eapply in_map. now eapply nthN_In; eauto.
-          now apply reach'_extensive.
-        * eapply Included_trans.
-          eapply env_locs_monotonic. now apply occurs_free_Eproj_Included.
-          eapply Included_trans. eapply env_locs_set_Inlcuded.
-          eapply Union_Included; [| eassumption ].
-          eapply Included_trans; [| now eapply reachable_in_dom; eauto ].
-          intros l1 Hin. eexists 1. split.
-          now constructor.
-          eexists l. eexists. repeat split; eauto; simpl.
-          eexists; split; eauto. now rewrite Hgety.
-          eapply In_Union_list; [| eassumption ].
-          eapply in_map. now eapply nthN_In; eauto.
-        * eapply Included_trans.
-          eapply env_locs_monotonic. now apply occurs_free_Eproj_Included.
-          eapply Included_trans. eapply env_locs_set_Inlcuded.
-          eapply Union_Included; [| eassumption ].
-          eapply Included_trans; [| now eapply reachable_in_dom; eauto ].
-          intros l1 Hin. eexists 1. split.
-          now constructor.
-          eexists l0. eexists. repeat split; eauto; simpl.
-          exists y; split; eauto. now rewrite Hgety0.
-          eapply In_Union_list; [| eassumption ].
-          eapply in_map. now eapply nthN_In; eauto.
-        * eapply heap_env_equiv_set.
-          eapply heap_env_equiv_antimon. eassumption.
-          eapply Setminus_Included_Included_Union. now eapply occurs_free_Eproj_Included.
-          eapply Heq in Hgety0. 
-          destruct Hgety0 as [l2' [Hget' Heq']]. subst_exp.
-          { rewrite res_equiv_eq in Heq'. simpl in Heq'.
-            rewrite Hgetl, Hgetl0 in Heq'.  destruct Heq' as [_ Hall].
-            symmetry.
-            eapply Forall2_nthN' with (v1 := v0) (v2 := v) in Hall.
-            eapply Hall; eassumption. eassumption. eassumption. }
-          { eapply occurs_free_Eproj... }
-      + (* D2 : Eval_GC *)
-        assert (Hex : exists  (Hbs1' : big_step H rho (Eproj x t n y e) (Res r1') c m0), size_big_step Hbs1' = S (size_big_step Hbs1)).
-        { exists (Eval_proj H rho x t n y e l v vs (Res r1') c m0 Hcost Hgety Hgetl Hargs Hbs1).
-          reflexivity. }
-        destruct Hex as [Hbs1' Hsize'].
-        eapply IH2 with (Hbs2 := Hbs2) (Hbs1 := Hbs1');
-          [ | | | | | reflexivity | | reflexivity | reflexivity | ]; try eassumption.
-        * omega.
-        * eapply heap_equiv_respects_well_formed; [| eassumption ].
-          destruct Hgc as [_ Hequiv]. exact Hequiv.
-        * eapply heap_equiv_in_dom.
-          destruct Hgc as [_ Hequiv]. exact Hequiv.
-          reflexivity. eassumption.
-        * intros. subst. eapply IH1 with (Hbs1 := Hbs0);
-            [| | | | | reflexivity | | reflexivity | reflexivity |]; try eassumption.
-          omega.
-        * edestruct Equivalence_heap_env_equiv. eapply Equivalence_Transitive; eauto.
-          eapply heap_env_equiv_heap_equiv.
-          eapply collect_heap_eq. eassumption.
-    - (* D1 : Eval_case *)
-      subst m. remember (Ecase y cl) as e'. destruct Hbs2; inv Heqe'; simpl in *.
-      + (* D2 : OOT *) discriminate.
-      + (* D2 : Eval_case *)
-        eapply Heq in Hgety. edestruct Hgety as [l' [Hget Heql']].
-        subst_exp. rewrite res_equiv_eq in Heql'. simpl in Heql'.
-        rewrite Hgetl, Hgetl0 in Heql'. destruct Heql' as [Heqt Hall]. subst.
-        subst_exp.
-        eapply IH1 with (Hbs1 := Hbs1);
-          [ | | | | | reflexivity | | reflexivity | reflexivity | ]; try eassumption; eauto.
-        * eapply well_formed_antimon; [| eassumption ].
-          eapply reach'_set_monotonic. eapply env_locs_monotonic.
-          rewrite occurs_free_Ecase_Included. reflexivity.
-          eapply cps_util.findtag_In. eassumption.
-        * eapply well_formed_antimon; [| eassumption ].
-          eapply reach'_set_monotonic. eapply env_locs_monotonic.
-          rewrite occurs_free_Ecase_Included. reflexivity.
-          eapply cps_util.findtag_In. eassumption.
-        * eapply Included_trans; [| eassumption ].
-          eapply env_locs_monotonic.
-          rewrite occurs_free_Ecase_Included. reflexivity.
-          eapply cps_util.findtag_In. eassumption.
-        * eapply Included_trans; [| eassumption ].
-          eapply env_locs_monotonic.
-          rewrite occurs_free_Ecase_Included. reflexivity.
-          eapply cps_util.findtag_In. eassumption.
-        * eapply heap_env_equiv_antimon.
-          eassumption.
-          rewrite occurs_free_Ecase_Included. reflexivity.
-          eapply cps_util.findtag_In. eassumption.
-        * eauto.
-      + (* D2 : Eval_GC *)
-        assert (Hex : exists  (Hbs1' : big_step H rho (Ecase y cl) (Res r1') c m0), size_big_step Hbs1' = S (size_big_step Hbs1)).
-        { exists (Eval_case H rho y cl l t vs e (Res r1') c m0 Hcost Hgety Hgetl Hfind Hbs1). reflexivity. }
-        destruct Hex as [Hbs1' Hsize'].
-        eapply IH2 with (Hbs2 := Hbs2) (Hbs1 := Hbs1');
-          [ | | | | | reflexivity | | reflexivity | reflexivity | ]; try eassumption.
-        * omega.
-        * eapply heap_equiv_respects_well_formed; [| eassumption ].
-          destruct Hgc as [_ Hequiv]. exact Hequiv.
-        * eapply heap_equiv_in_dom.
-          destruct Hgc as [_ Hequiv]. exact Hequiv.
-          reflexivity. eassumption.
-        * intros. subst.
-          eapply IH1 with (Hbs1 := Hbs0);
-            [| | | | | reflexivity | | reflexivity | reflexivity |]; try eassumption.
-          omega.
-        * edestruct Equivalence_heap_env_equiv. eapply Equivalence_Transitive; eauto.
-          eapply heap_env_equiv_heap_equiv.
-          eapply collect_heap_eq. eassumption.
-    - (* D1 : Eval_fun *)
-      subst m. remember (Efun B e) as e'. destruct Hbs2; inv Heqe'; simpl in *.
-      + (* D2 : OOT *) discriminate.
-      + (* D2 : Eval_fun *) 
-        eapply IH1 with (Hbs1 := Hbs1);
-        [| | | | | reflexivity | | reflexivity | reflexivity | ]; try eassumption.
-        * omega.
-        * eapply well_formed_antimon. eapply reach'_set_monotonic.
-          eapply env_locs_monotonic. now apply occurs_free_Efun_Included.
-          eapply well_formed_reach_alloc_def_funs; [ | | | | eassumption ].
-          eapply well_formed_alloc; [| eassumption | ]. 
-          rewrite <- well_formed_reach_alloc_same; eassumption.
-          eapply Included_trans. eapply restrict_env_env_locs. eassumption.
-          eapply Included_trans; [ | eassumption ].
-          eapply env_locs_monotonic. normalize_occurs_free...
-          eapply Included_trans; [ eassumption |].
-          now eapply dom_subheap; eapply alloc_subheap; eauto.
-          now erewrite gas; eauto.
-          eapply Included_trans; [| now eapply reach'_extensive ].
-          eapply Included_trans. eapply restrict_env_env_locs. eassumption.
-          eapply env_locs_monotonic. normalize_occurs_free...
-        * eapply well_formed_antimon. eapply reach'_set_monotonic.
-          eapply env_locs_monotonic. now apply occurs_free_Efun_Included.
-          eapply well_formed_reach_alloc_def_funs; [ | | | | eassumption ].
-          eapply well_formed_alloc; [| eassumption | ]. 
-          rewrite <- well_formed_reach_alloc_same; eassumption.
-          eapply Included_trans. eapply restrict_env_env_locs. eassumption.
-          eapply Included_trans; [ | eassumption ].
-          eapply env_locs_monotonic. normalize_occurs_free...
-          eapply Included_trans; [ eassumption |].
-          now eapply dom_subheap; eapply alloc_subheap; eauto.
-          now erewrite gas; eauto.
-          eapply Included_trans; [| now eapply reach'_extensive ].
-          eapply Included_trans. eapply restrict_env_env_locs. eassumption.
-          eapply env_locs_monotonic. normalize_occurs_free...
-        * eapply Included_trans. eapply env_locs_monotonic. now apply occurs_free_Efun_Included.
-          eapply def_closures_env_locs_in_dom; [eassumption | ].
-          eapply Included_trans. eassumption.
-          eapply dom_subheap. now eapply alloc_subheap; eauto.
-        * eapply Included_trans. eapply env_locs_monotonic. now apply occurs_free_Efun_Included.
-          eapply def_closures_env_locs_in_dom; [eassumption | ].
-          eapply Included_trans. eassumption.
-          eapply dom_subheap. now eapply alloc_subheap; eauto.
-        * eapply heap_env_equiv_antimon with (S1 := occurs_free (Efun B e) :|: name_in_fundefs B);
-          [| now apply occurs_free_Efun_Included ].
-          setoid_rewrite <- Hfuns0. setoid_rewrite <- Hfuns.
-          eapply heap_env_equiv_def_funs.
-          (* closed H' *)
-          eapply reach'_closed. rewrite reach'_alloc; [ | eassumption | ].
-          eapply well_formed_alloc. eassumption. eassumption.
-          eapply Included_trans. eapply restrict_env_env_locs. eassumption.
-          eapply Included_trans; [| eassumption ].
-          eapply env_locs_monotonic. normalize_occurs_free...
-          eapply Included_trans; [| now eapply reach'_extensive ].
-          eapply Included_trans. eapply restrict_env_env_locs. eassumption.
-          eapply env_locs_monotonic. normalize_occurs_free...
-          eapply Included_trans. eassumption. eapply dom_subheap.
-          eapply alloc_subheap. eassumption.
-          (* closed H0' *)
-          eapply reach'_closed. rewrite reach'_alloc; [ | eassumption | ].
-          eapply well_formed_alloc. eassumption. eassumption.
-          eapply Included_trans. eapply restrict_env_env_locs. eassumption.
-          eapply Included_trans; [| eassumption ].
-          eapply env_locs_monotonic. normalize_occurs_free...
-          eapply Included_trans; [| now eapply reach'_extensive ].
-          eapply Included_trans. eapply restrict_env_env_locs. eassumption.
-          eapply env_locs_monotonic. normalize_occurs_free...
-          eapply Included_trans. eassumption. eapply dom_subheap.
-          eapply alloc_subheap. eassumption.
-          (* env locs rho \subset reach H' *)
-          eapply Included_trans; [| now apply reach'_extensive ].
-          eapply env_locs_monotonic...
-          (* env locs rho0 \subset reach H'0 *)
-          eapply Included_trans; [| now apply reach'_extensive ].
-          eapply env_locs_monotonic...
-          (* get env_loc H' *)
-          now erewrite gas; eauto.
-          (* get env_loc0 H'0 *)
-          now erewrite gas; eauto.
-          (* env locs rho_clo \subset reach H' *)
-          eapply Included_trans. eapply restrict_env_env_locs. eassumption.
-          eapply Included_trans; [| now apply reach'_extensive ].
-          normalize_occurs_free...
-          (* env locs rho_clo0 \subset reach H0' *)
-          eapply Included_trans. eapply restrict_env_env_locs. eassumption.
-          eapply Included_trans; [| now apply reach'_extensive ].
-          normalize_occurs_free...
-          (* fv subset *)
-          rewrite Setminus_Union_distr.
-          rewrite Setminus_Disjoint. normalize_occurs_free...
-          normalize_occurs_free. eapply Union_Disjoint_l.
-          eapply Disjoint_sym. now apply occurs_free_fundefs_name_in_fundefs_Disjoint.
-          eapply Disjoint_Setminus_l. reflexivity.
-          (* (Loc env_loc, H') ≈ (Loc env_loc0, H'0) *)
-          rewrite res_equiv_eq. simpl.
-          erewrite gas; [| eassumption ]. erewrite gas; [| eassumption ]. 
-          (* |- (H', rho) ⩪ (H'0, rho0) *)
-          eapply heap_env_equiv_restrict_env; [| | eassumption | eassumption ].
-          eapply heap_env_equiv_weaking_cor; try eassumption.
-          eapply alloc_subheap; eassumption.
-          eapply alloc_subheap; eassumption.
-          normalize_occurs_free...
-          eapply heap_env_equiv_antimon with (S1 := occurs_free (Efun B e));
-            [| now eauto with Ensembles_DB ].
-          eapply heap_env_equiv_weaking_cor; try eassumption.
-          eapply alloc_subheap; eassumption.
-          eapply alloc_subheap; eassumption.
-      + (* D2 : Eval_GC *)
-        assert (Hex : exists  (Hbs1' : big_step H rho (Efun B e) (Res r1') c m0), size_big_step Hbs1' = S (size_big_step Hbs1)).
-        { exists (Eval_fun H H' H'' rho rho_clo rho' B env_loc e (Res r1') c m0 Hcost Hres Halloc Hfuns Hbs1).
-          reflexivity. }
-        destruct Hex as [Hbs1' Hsize'].
-        eapply IH2 with (Hbs2 := Hbs2) (Hbs1 := Hbs1'); [| | |  | | reflexivity | | reflexivity | reflexivity | ]; try eassumption.
-        * omega.
-        * eapply heap_equiv_respects_well_formed; [| eassumption ].
-          destruct Hgc as [_ Hequiv]. exact Hequiv.
-        * eapply heap_equiv_in_dom.
-          destruct Hgc as [_ Hequiv]. exact Hequiv.
-          reflexivity. eassumption.
-        * intros. subst.
-          eapply IH1 with (Hbs1 := Hbs0);
-            [| | | | | reflexivity | | reflexivity | reflexivity |]; try eassumption.
-          omega.
-        * edestruct Equivalence_heap_env_equiv. eapply Equivalence_Transitive; eauto.
-          eapply heap_env_equiv_heap_equiv.
-          eapply collect_heap_eq. eassumption.
-    - (* D1 : Eval_app *)
-      subst m. remember (Eapp f t ys) as e'. destruct Hbs2; inv Heqe'; simpl in *.
-      + (* D2 : OOT *) discriminate.
-      + (* D2 : Eval_app *)
-        assert (Hgetf' := Hgetf). assert (Hgetl' := Hgetl).
-        eapply Heq in Hgetf; [| normalize_occurs_free; now eauto with Ensembles_DB ].
-        destruct Hgetf as [l' [Hget Hequiv]]. repeat subst_exp.
-        rewrite res_equiv_eq in Hequiv. simpl in Hequiv.
-        rewrite Hgetl, Hgetl0 in Hequiv. destruct Hequiv as [Hv1 Hv2].
-        rewrite res_equiv_eq in Hv1, Hv2.
-        simpl in Hv1, Hv2. inv Hv1. rewrite Hget_env, Hget_env0 in Hv2. 
-        repeat subst_exp.
-        assert (Henv1 :  env_locs rho_clo (Full_set var) \subset
-                         reach' H (env_locs rho (occurs_free (Eapp f t ys)))).
-        { normalize_occurs_free. rewrite env_locs_Union, reach'_Union.
-          eapply Included_Union_preserv_r.
-          eapply Included_trans; [| now eapply Included_post_n_reach' with (n := 2) ].
-          simpl. rewrite env_locs_Singleton; try eassumption. simpl. rewrite post_Singleton; try eassumption.
-          simpl. rewrite Union_Empty_set_neut_l.
-          rewrite post_Singleton; try eassumption. eapply env_locs_monotonic... }
-        assert (Henv2 :  env_locs rho_clo0 (Full_set var) \subset
-                         reach' H0 (env_locs rho0 (occurs_free (Eapp f t ys)))).
-        { normalize_occurs_free. rewrite env_locs_Union, reach'_Union.
-          eapply Included_Union_preserv_r.
-          eapply Included_trans; [| now eapply Included_post_n_reach' with (n := 2) ].
-          simpl. rewrite env_locs_Singleton; try eassumption. simpl. rewrite post_Singleton; try eassumption.
-          simpl. rewrite Union_Empty_set_neut_l.
-          rewrite post_Singleton; try eassumption. eapply env_locs_monotonic... }
-        assert (Hvs1 : Union_list (map val_loc vs) \subset
-                       env_locs rho (occurs_free (Eapp f t ys))).
-        { rewrite <- env_locs_FromList; eauto. normalize_occurs_free.
-          eapply env_locs_monotonic... }
-        assert (Hvs2 : Union_list (map val_loc vs0) \subset
-                       env_locs rho0 (occurs_free (Eapp f t ys))).
-        { rewrite <- env_locs_FromList; eauto. normalize_occurs_free.
-          eapply env_locs_monotonic... }
-        eapply IH1 with (rho1 := rho_clo2) (rho2 := rho_clo4) (Hbs1 := Hbs1);
-          [| | | | | reflexivity | | reflexivity | reflexivity | ]; try eassumption.
-        * omega.
-        * { eapply well_formed_antimon. 
-            - eapply reach'_set_monotonic. eapply env_locs_monotonic.
-              eapply occurs_free_in_fun.
-              eapply find_def_correct. eassumption.
-            - rewrite Union_commut.
-              eapply well_formed_antimon.
-              eapply reach'_set_monotonic. eapply env_locs_monotonic.
-              eapply Included_Union_compat.
-              eapply Included_Union_compat with (s2' := Full_set _); [ reflexivity |]...
-              reflexivity.
-              eapply well_formed_reach_setlist; [| | eassumption ].
-              + rewrite Union_commut.
-                eapply well_formed_reach_alloc_def_funs; try eassumption.
-                * eapply well_formed_antimon; [| eassumption ].
-                  eapply Included_trans; [| now eapply reach'_idempotent ]. 
-                  eapply reach'_set_monotonic. eassumption.
-                * eapply Included_trans; [| eapply reachable_in_dom; eassumption ].
-                  eassumption.
-                * eapply reach'_extensive.
-              + eapply well_formed_def_funs; [| now eexists; eauto | now eauto ]. 
-                rewrite <- well_formed_reach_def_closed_same; [| | | | eassumption ].
-                eapply well_formed_antimon; [| eassumption ].
-                eapply reach'_set_monotonic. eassumption.
-                eapply well_formed_antimon; [| eassumption ].
-                eapply reach'_set_monotonic. eassumption.
-                now eexists; eauto.
-                eapply Included_trans; eauto. }
-        * { eapply well_formed_antimon. 
-            - eapply reach'_set_monotonic. eapply env_locs_monotonic.
-              eapply occurs_free_in_fun.
-              eapply find_def_correct. eassumption.
-            - rewrite Union_commut.
-              eapply well_formed_antimon.
-              eapply reach'_set_monotonic. eapply env_locs_monotonic.
-              eapply Included_Union_compat.
-              eapply Included_Union_compat with (s2' := Full_set _); [ reflexivity |]...
-              reflexivity.
-              eapply well_formed_reach_setlist; [| | eassumption ].
-              + rewrite Union_commut.
-                eapply well_formed_reach_alloc_def_funs; [| | | | eassumption]; try eassumption.
-                * eapply well_formed_antimon; [| eassumption ].
-                  eapply Included_trans; [| now eapply reach'_idempotent ]. 
-                  eapply reach'_set_monotonic. eassumption.
-                * eapply Included_trans; [| eapply reachable_in_dom; eassumption ].
-                  eassumption.
-                * eapply reach'_extensive.
-              + eapply well_formed_def_funs; [| | now eauto ]; try (now eexists; eauto). 
-                rewrite <- well_formed_reach_def_closed_same; [| | | | eassumption ].
-                eapply well_formed_antimon; [| eassumption ].
-                eapply reach'_set_monotonic. eassumption.
-                eapply well_formed_antimon; [| eassumption ].
-                eapply reach'_set_monotonic. eassumption.
-                now eexists; eauto.
-                eapply Included_trans; eauto. }
-        * eapply Included_trans. eapply env_locs_monotonic. eapply occurs_free_in_fun.
-          eapply find_def_correct. eassumption. rewrite Union_commut.
-          eapply Included_trans. eapply env_locs_setlist_Included; eauto.
-          eapply Union_Included.
-          rewrite Union_commut.
-          eapply def_closures_env_locs_in_dom; try eassumption.
-          eapply Included_trans; [| eapply reachable_in_dom; eassumption ].
-          eapply Included_trans; [| now apply Henv1 ].
-          eapply env_locs_monotonic...
-          eapply Included_trans; [| eapply dom_subheap; eapply def_funs_subheap; now eauto ].
-          eapply Included_trans; eassumption.
-        * eapply Included_trans. eapply env_locs_monotonic. eapply occurs_free_in_fun.
-          eapply find_def_correct. eassumption. rewrite Union_commut.
-          eapply Included_trans. eapply env_locs_setlist_Included; eauto.
-          eapply Union_Included.
-          rewrite Union_commut.
-          eapply def_closures_env_locs_in_dom; try eassumption.
-          eapply Included_trans; [| eapply reachable_in_dom; eassumption ].
-          eapply Included_trans; [| now apply Henv2 ].
-          eapply env_locs_monotonic...
-          eapply Included_trans; [| eapply dom_subheap; eapply def_funs_subheap; now eauto ].
-          eapply Included_trans; eassumption.
-        * { eapply heap_env_equiv_setlist; try eassumption.
-            + eapply heap_env_equiv_antimon with (S1 := occurs_free_fundefs B0 :|: name_in_fundefs B0);
-              [| eapply Included_trans;
-                 [ eapply Included_Setminus_compat;
-                   [eapply occurs_free_in_fun; eapply find_def_correct; eassumption | reflexivity ]
-                 | now eauto with Ensembles_DB ]].
-              setoid_rewrite <- Hredef. setoid_rewrite <- Hredef0.
-              eapply heap_env_equiv_def_funs; try eassumption.
-              * eapply reach'_closed; eassumption.
-              * eapply reach'_closed; eassumption.
-              * eapply Included_trans; [| now apply Henv1 ].
-                eapply env_locs_monotonic...
-              * eapply Included_trans; [| now apply Henv2 ].
-                eapply env_locs_monotonic...
-              * rewrite Setminus_Union_distr.
-                rewrite Setminus_Disjoint. now eauto with Ensembles_DB.
-                eapply Disjoint_sym. now apply occurs_free_fundefs_name_in_fundefs_Disjoint.
-              * rewrite res_equiv_eq. simpl. rewrite Hget_env, Hget_env0.
-                eassumption.
-              * eapply heap_env_equiv_antimon; [ eassumption | ]... 
-            + eapply heap_env_equiv_getlist_Forall2; eauto.
-              eapply heap_env_equiv_weaking_cor; try eassumption.
-              eapply def_funs_subheap. now eauto.
-              eapply def_funs_subheap. now eauto. normalize_occurs_free... }
-      + (* D2 : Eval_GC *)
-        assert (Hex : exists (Hbs1' : big_step H rho (Eapp f t ys) (Res r1') c m0),
-                        size_big_step Hbs1' = S (size_big_step Hbs1)).
-        { exists (Eval_app H H' rho rho_clo rho_clo1 rho_clo2 B f f' t xs e l env_loc vs ys (Res r1') c m0 Hcost Hgetf Hgetl Hget_env Hfind Hargs Hredef Hset Hbs1).
-          reflexivity. }
-        destruct Hex as [Hbs1' Hsize'].
-        eapply IH2 with (Hbs2 := Hbs2) (Hbs1 := Hbs1');
-          [| | | | | reflexivity | | reflexivity | reflexivity | ]; try eassumption.
-        * omega.
-        * eapply heap_equiv_respects_well_formed; [| eassumption ].
-          destruct Hgc as [_ Hequiv]. exact Hequiv.
-        * eapply heap_equiv_in_dom.
-          destruct Hgc as [_ Hequiv]. exact Hequiv.
-          reflexivity. eassumption.
-        * intros. subst.
-          eapply IH1 with (Hbs1 := Hbs0); [| | | | | reflexivity | | reflexivity | reflexivity | ]; try eassumption.
-          omega.
-        * edestruct Equivalence_heap_env_equiv. eapply Equivalence_Transitive; eauto.
-          eapply heap_env_equiv_heap_equiv. eapply collect_heap_eq. eassumption.      
-    - (* D1 : Eval_halt *)
-      subst m. remember (Ehalt x) as e'. destruct Hbs2; inv Heqe'; simpl in *.
-      + (* D2 : OOT *) discriminate.
-      + (* D2 : Eval_halt *)
-        eapply Heq in Hget; eauto. destruct Hget as [l' [Hget Hequiv]].
-        inv Heq1; inv Heq2. subst_exp. eassumption.
-      + (* D2 : Eval_GC *)
-        assert (Hex : exists  (Hbs1' : big_step H rho (Ehalt x) (Res (v, H)) c (size_heap H)), size_big_step Hbs1' = 0).
-        { exists (Eval_halt H rho x v c (size_heap H) Hcost Hget eq_refl). eauto. }
-        destruct Hex as [Hbs1' Hsize'].
-        inv Heq1.
-        eapply IH2 with (Hbs2 := Hbs2) (Hbs1 := Hbs1');
-          [| | | | | reflexivity | | reflexivity | reflexivity | ]; try eassumption.
-        * omega.
-        * eapply heap_equiv_respects_well_formed; [| eassumption ].
-          destruct Hgc as [_ Hequiv]. exact Hequiv.
-        * eapply heap_equiv_in_dom.
-          destruct Hgc as [_ Hequiv]. exact Hequiv.
-          reflexivity. eassumption.
-        * intros. subst. eapply IH1 with (Hbs1 := Hbs1);
-            [| | | | | reflexivity | | reflexivity | reflexivity | ]; try eassumption.
-          omega. 
-        * edestruct Equivalence_heap_env_equiv. eapply Equivalence_Transitive; eauto.
-          eapply heap_env_equiv_heap_equiv.
-          eapply collect_heap_eq. eassumption.
-    - (* D1 : Eval_GC *)
-      eapply IH1 with (Hbs1 := Hbs1); [| | | | | reflexivity | eassumption | | | ].
-      + omega.
-      + eapply heap_equiv_respects_well_formed; [| eassumption ].
-        destruct Hgc as [_ Hequiv]. exact Hequiv.
-      + eassumption.
-      + eapply heap_equiv_in_dom.
-        destruct Hgc as [_ Hequiv]. exact Hequiv.
-        reflexivity. eassumption.
-      + eassumption.
-      + eassumption.
-      + eassumption.
-      + edestruct Equivalence_heap_env_equiv. eapply Equivalence_Transitive; try eassumption.
-        symmetry. eapply heap_env_equiv_heap_equiv.
-        eapply collect_heap_eq. eassumption.
+  Fixpoint costCC_ctx (c : exp_ctx) : nat :=
+    match c with
+      | Econstr_c x t ys c => 1 + length ys
+      | Eproj_c x t n y c => 1 
+      | Efun1_c B c => 1
+      | Eprim_c x p ys c => 1 + length ys
+      | Hole_c => 0
+      | Efun2_c _ _ => 0 (* maybe fix but not needed for now *)
+      | Ecase_c _ _ _ _ _ => 0
+    end.
+
+  Inductive ctx_to_heap_env : exp_ctx -> heap block -> env -> heap block -> env -> nat -> Prop :=
+  | Hole_c_to_heap_env :
+      forall H rho,
+        ctx_to_heap_env Hole_c H rho H rho 0
+  | Econstr_c_to_rho :
+      forall H H' H'' rho rho' x t ys C vs l c,
+        getlist ys rho = Some vs ->
+        alloc (Constr t vs) H = (l, H') ->
+        
+        ctx_to_heap_env C H' (M.set x (Loc l) rho)  H'' rho'  c -> 
+        
+        ctx_to_heap_env (Econstr_c x t ys C) H rho H'' rho' (c + costCC_ctx (Econstr_c x t ys C))
+
+  | Eproj_c_to_rho :
+      forall H H' rho rho' x N t y C vs v t' l c,
+        
+        M.get y rho = Some (Loc l) ->
+        get l H = Some (Constr t' vs) ->
+        nthN vs N = Some v ->
+        
+        ctx_to_heap_env C H (M.set x v rho)  H' rho'  c -> 
+        
+        ctx_to_heap_env (Eproj_c x t N y C) H rho H' rho' (c + costCC_ctx (Eproj_c x t N y C)).
+  
+
+  (** Allocation cost of an evaluation context *)
+  Fixpoint cost_alloc_ctx (c : exp_ctx) : nat :=
+    match c with
+      | Econstr_c x t ys c => 1 + length ys + cost_alloc_ctx c
+      | Eproj_c x t n y c => cost_alloc_ctx c
+      (* not relevant *)
+      | Efun1_c B c => cost_alloc_ctx c
+      | Eprim_c x p ys c => cost_alloc_ctx c
+      | Hole_c => 0
+      | Efun2_c f _ => cost_alloc_f_ctx f
+      | Ecase_c _ _ _ c _ => cost_alloc_ctx c
+    end
+  with
+  cost_alloc_f_ctx (f : fundefs_ctx) : nat :=
+    match f with
+      | Fcons1_c _ _ _ c _ => cost_alloc_ctx c
+      | Fcons2_c _ _ _ _ f => cost_alloc_f_ctx f
+    end.
+  
+  Lemma cost_alloc_ctx_comp_ctx_f C C' :
+    cost_alloc_ctx (comp_ctx_f C C') =
+    cost_alloc_ctx C + cost_alloc_ctx C'
+  with cost_alloc_comp_f_ctx_f f C' :
+         cost_alloc_f_ctx (comp_f_ctx_f f C') =
+         cost_alloc_f_ctx f + cost_alloc_ctx C'.
+  Proof.
+    - destruct C; simpl; try reflexivity;
+      try (rewrite cost_alloc_ctx_comp_ctx_f; omega).
+      rewrite cost_alloc_comp_f_ctx_f. omega.
+    - destruct f; simpl; try reflexivity.
+      rewrite cost_alloc_ctx_comp_ctx_f; omega.
+      rewrite cost_alloc_comp_f_ctx_f. omega.
+  Qed. 
+
+    (** * Lemmas about [ctx_to_heap_env] *)
+
+  Lemma ctx_to_heap_env_comp_ctx_f_r C1 C2 rho1 H1 m1 rho2 H2 m2 rho3 H3 :
+    ctx_to_heap_env C1 H1 rho1 H2 rho2 m1 ->
+    ctx_to_heap_env C2 H2 rho2 H3 rho3 m2 ->
+    ctx_to_heap_env (comp_ctx_f C1 C2) H1 rho1 H3 rho3 (m1 + m2).
+  Proof.
+    revert C2 rho1 H1 m1 rho2 H2 m2 rho3 H3.
+    induction C1; intros C2 rho1 H1 m1 rho2 H2 m2 rho3 H3 Hctx1 GHctx2; inv Hctx1.
+    - eassumption.
+    - replace (c0 + costCC_ctx (Econstr_c v c l C1) + m2) with (c0 + m2 + costCC_ctx (Econstr_c v c l C1)) by omega.
+      simpl. econstructor; eauto. 
+    - replace (c0 + costCC_ctx (Eproj_c v c n v0 C1) + m2) with (c0 + m2 + costCC_ctx (Eproj_c v c n v0 C1)) by omega.
+      simpl. econstructor; eauto.
   Qed.
 
-  *)
+  Lemma ctx_to_heap_env_comp_ctx_l C C1 C2 H rho H' rho' m :
+    ctx_to_heap_env C H rho H' rho' m ->
+    comp_ctx C1 C2 C ->
+    exists rho'' H'' m1 m2,
+      ctx_to_heap_env C1 H rho H'' rho'' m1 /\
+      ctx_to_heap_env C2 H'' rho'' H' rho' m2 /\
+      m = m1 + m2.
+  Proof.
+    intros Hctx. revert C1 C2.
+    induction Hctx; intros C1 C2 Hcomp.
+    - inv Hcomp. repeat eexists; constructor.
+    - inv Hcomp.
+      + edestruct IHHctx as [rho'' [H''' [m1 [m2 [Hc1 [Hc2 Hadd]]]]]].
+        constructor. inv H1.
+        do 4 eexists. split; [ | split ].  econstructor.
+        econstructor; eauto. omega.
+      + edestruct IHHctx as [rho'' [H''' [m1 [m2 [Hc1 [Hc2 Hadd]]]]]].
+        eassumption.
+        do 4 eexists. split; [ | split ]. econstructor; eauto.
+        eassumption. simpl. omega.
+    - inv Hcomp.
+      + edestruct IHHctx as [rho'' [H''' [m1 [m2 [Hc1 [Hc2 Hadd]]]]]].
+        constructor. inv H1.
+        do 4 eexists; split; [| split ]. constructor.
+        econstructor; eauto. omega.
+      + edestruct IHHctx as [rho'' [H''' [m1 [m2 [Hc1 [Hc2 Hadd]]]]]].
+        eassumption.
+        do 4 eexists; split; [| split ]. econstructor; eauto.
+        eassumption. simpl. omega.
+  Qed.
+
+  Lemma ctx_to_heap_env_comp_ctx_f_l C1 C2 H rho H' rho' m :
+    ctx_to_heap_env (comp_ctx_f C1 C2) H rho H' rho' m ->
+    exists rho'' H'' m1 m2,
+      ctx_to_heap_env C1 H rho H'' rho'' m1 /\
+      ctx_to_heap_env C2 H'' rho'' H' rho' m2 /\
+      m = m1 + m2.
+  Proof.
+    intros. eapply ctx_to_heap_env_comp_ctx_l. eassumption.
+    eapply comp_ctx_f_correct. reflexivity.
+  Qed.
+
+  Lemma ctx_to_heap_env_size_heap C rho1 rho2 H1 H2 c :
+    ctx_to_heap_env C H1 rho1 H2 rho2 c ->
+    size_heap H2 = size_heap H1 + cost_alloc_ctx C. 
+  Proof.
+    intros Hctx; induction Hctx; eauto.
+    simpl. rewrite IHHctx.
+    unfold size_heap.
+    erewrite (HL.size_with_measure_alloc _ _ _ H H');
+      [| reflexivity | eassumption ].
+    erewrite getlist_length_eq; [| eassumption ]. 
+    simpl. omega.
+  Qed.
+
+  Lemma ctx_to_heap_env_subheap C H rho H' rho' m :
+    ctx_to_heap_env C H rho H' rho' m ->
+    H ⊑ H'.
+  Proof.
+    intros Hc; induction Hc.
+    - eapply HL.subheap_refl.
+    - eapply HL.subheap_trans.
+      eapply HL.alloc_subheap. eassumption. eassumption.
+    - eassumption.
+  Qed.  
+  
 
 End SpaceSem.
